src/PlutusIR/Semantics/Static/normaliser_STLC/gu_naive/TypeSubstitutionSOP.v
@@ -1,0 +1,215 @@
+From Equations Require Import Equations.
+From PlutusCert Require Import PlutusIRSOP.
+
+From PlutusCert Require Import plutus_util util.
+
+Require Import Coq.Strings.String.
+Local Open Scope string_scope.
+Require Import Coq.Lists.List.
+Local Open Scope list_scope.
+Import ListNotations.
+
+
+(** * Regular substitution of types *)
+
+Fixpoint substituteT (X : string) (U T : ty) : ty :=
+  match T with
+  | Ty_Var Y =>
+    if X =? Y then U else Ty_Var Y
+  | Ty_Fun T1 T2 =>
+    Ty_Fun (substituteT X U T1) (substituteT X U T2)
+  | Ty_IFix F T =>
+    Ty_IFix (substituteT X U F) (substituteT X U T)
+  | Ty_Forall Y K T' =>
+    if X =? Y then Ty_Forall Y K T' else Ty_Forall Y K (substituteT X U T')
+  | Ty_Builtin u =>
+    Ty_Builtin u
+  | Ty_Lam Y K1 T' =>
+    if X =? Y then Ty_Lam Y K1 T' else Ty_Lam Y K1 (substituteT X U T')
+  | Ty_App T1 T2 =>
+    Ty_App (substituteT X U T1) (substituteT X U T2)
+  | Ty_SOP Tss =>
+    Ty_SOP (map (substituteT X U) Tss)
+  end.
+
+(** Multi-substitutions of types*)
+Fixpoint msubstT (ss : list (string * ty)) (T : ty) : ty :=
+  match ss with
+  | nil => T
+  | (a, T0) :: ss' => msubstT ss' (substituteT a T0 T)
+  end.
+
+(** * Capture-avoiding substitution of types *)
+Require Import Lia.
+Import ListNotations.
+
+(* Moved from analysis.freevars*)
+  Function ftv (T : ty) : list string :=
+    match T with
+    | Ty_Var X =>
+        [X]
+    | Ty_Fun T1 T2 =>
+        ftv T1 ++ ftv T2
+    | Ty_IFix F T =>
+        ftv F ++ ftv T
+    | Ty_Forall X K T' =>
+        remove string_dec X (ftv T')
+    | Ty_Builtin u =>
+        []
+    | Ty_Lam X K1 T' =>
+        remove string_dec X (ftv T')
+    | Ty_App T1 T2 =>
+        ftv T1 ++ ftv T2
+    | Ty_SOP Tss =>
+        concat (map ftv Tss)
+    end.
+
+
+(** Assume that we compute the substitution of U for X in (LamAbs Y K T).
+    We reduce the  problem of generating a fresh type variable to generating
+    a type variable A such that:
+
+    A <> X /\ ~ In A (ftv U) /\ ~ In A (ftv T)
+
+    We generate a ``fresh'' type variable naively: We concatenate X, all
+    free type variables in U and all free type variables in T together.
+    By appending an arbitrary letter such as "a" to the result of the previous,
+    we get a type variable string which is strictly larger than [X], the
+    free type variables in U and the free type variables in T. This means
+    that the abovementioned formula holds.
+
+    TODO: The above is only an informal proof, so we should prove freshness
+    formally as well.
+*)
+Definition fresh (X : string) (U T : ty) : string :=
+  "a" ++ X ++ (Coq.Strings.String.concat EmptyString (ftv U)) ++ (Coq.Strings.String.concat EmptyString (ftv T)).
+
+Lemma fresh__X : forall X U T,
+    X <> fresh X U T.
+Proof with eauto.
+  intros. intros Hcon.
+  induction X; induction (ftv U); induction (ftv T).
+  all: simpl in Hcon.
+  all: inversion Hcon; subst...
+Qed.
+
+Lemma fresh__S : forall X U T,
+    ~ In (fresh X U T) (ftv U).
+Proof. Abort.
+
+Lemma fresh__T : forall X U T,
+    ~ In (fresh X U T) (ftv T).
+Proof. Abort.
+
+Definition rename (X Y : string) (T : ty) := substituteT X (Ty_Var Y) T.
+
+Fixpoint size (T : ty) : nat :=
+  match T with
+  | Ty_Var Y => 1
+  | Ty_Fun T1 T2 => 1 + size T1 + size T2
+  | Ty_IFix F T => 1 + size F + size T
+  | Ty_Forall bX K T0 => 1 + size T0
+  | Ty_Builtin u => 1
+  | Ty_Lam bX K T0 => 1 + size T0
+  | Ty_App T1 T2 => 1 + size T1 + size T2
+  (* | Ty_SOP Tss => 1 + fold_left (fun acc Ts => acc + fold_left (fun acc T => size T + acc) Ts 0) Tss 0 *)
+  | Ty_SOP Tss => 1 + fold_right (fun T acc => size T + acc) 0 Tss
+  (* NOTE: Using fold_right: easier to prove with in how it "spits" out a term that is "outside of"  the recursive fold_right*)
+  end.
+
+Lemma ty_sop_smaller : forall Tss T,
+  size T < size (Ty_SOP (T::Tss)).
+Proof.
+  simpl. lia.
+Qed.
+
+Lemma ty_sop_le2 : forall Tss T,
+  size (Ty_SOP Tss) <= size (Ty_SOP (T::Tss)).
+Proof.
+  intros. simpl. simpl.
+  remember ((fold_right
+  (fun (T0 : ty) (acc : nat) =>
+size T0 + acc)
+  0
+  Tss)) as fr.
+  lia.
+Qed.
+
+Lemma size_list_smaller : forall (T : ty) (Tss : list ty),
+  In T Tss -> size T < size (Ty_SOP Tss).
+Proof.
+  intros. induction Tss.
+  - inversion H.
+  - destruct H.
+    + subst. simpl. lia.
+    + specialize (IHTss H).
+      assert (size (Ty_SOP Tss) <= size (Ty_SOP (a :: Tss))).
+      { apply ty_sop_le2. }
+      lia.
+Qed.
+
+Lemma rename_preserves_size : forall T X Y,
+    size T = size (rename X Y T).
+Proof.
+  intros.
+  unfold rename.
+  apply PlutusIRSOP.ty__ind with (P := fun T => size T = size (substituteT X (Ty_Var Y) T)); intros; simpl; eauto.
+  all: try solve [destruct (X =? X0); simpl; eauto].
+  induction H; auto.
+  f_equal; simpl; auto. 
+Qed.
+
+(* A version of map that remembers list membership. Necessary in termination argument of substituteTCA*)
+Fixpoint map' {A B : Type} (xs : list A) : (forall x : A, In x xs -> B) -> list B :=
+  match xs with
+  | [] => fun _ => []
+  | x :: xs => fun f =>
+      f x ((or_introl (eq_refl : x = x)) : In x (x::xs)) :: map' xs (fun (y : A) (Hin : In y xs) => f y (or_intror Hin : In y (x :: xs)))
+  end.
+
+Equations? substituteTCA (X : string) (U T : ty) : ty by wf (size T) :=
+  substituteTCA X U (Ty_Var Y) =>
+      if X =? Y then U else Ty_Var Y ;
+  substituteTCA X U (Ty_Fun T1 T2) =>
+      Ty_Fun (substituteTCA X U T1) (substituteTCA X U T2) ;
+  substituteTCA X U (Ty_IFix F T) =>
+      Ty_IFix (substituteTCA X U F) (substituteTCA X U T) ;
+  substituteTCA X U (Ty_Forall Y K T) =>
+      if X =? Y
+        then
+          Ty_Forall Y K T
+        else
+          if existsb (eqb Y) (ftv U)
+            then
+              let Y' := fresh X U T in
+              let T' := rename Y Y' T in
+              Ty_Forall Y' K (substituteTCA X U T')
+            else
+              Ty_Forall Y K (substituteTCA X U T) ;
+  substituteTCA X U (Ty_Builtin u) =>
+      Ty_Builtin u ;
+  substituteTCA X U (Ty_Lam Y K T) =>
+      if X =? Y
+        then
+          Ty_Lam Y K T
+        else
+          if existsb (eqb Y) (ftv U)
+            then
+              let Y' := fresh X U T in
+              let T' := rename Y Y' T in
+              Ty_Lam Y' K (substituteTCA X U T')
+            else
+              Ty_Lam Y K (substituteTCA X U T) ;
+  substituteTCA X U (Ty_App T1 T2) =>
+      Ty_App (substituteTCA X U T1) (substituteTCA X U T2);
+  substituteTCA X U (Ty_SOP Tss) => Ty_SOP (map' Tss (fun T Hin => substituteTCA X U T))
+  .
+Proof.
+
+
+  all: try solve
+    [ lia
+    || replace T' with (rename Y Y' T); eauto; rewrite <- rename_preserves_size; eauto
+    ].
+    apply size_list_smaller. auto.
+Qed.
