src/PlutusIR/Semantics/Static/normaliser_STLC/gu_naive/plutus_util.v
@@ -1,0 +1,35 @@
+Require Import Coq.Lists.List.
+Require Import Coq.Strings.String.
+Local Open Scope string_scope.
+
+Definition map2 {A B : Type} (f : A -> B) (ll : list (list A)) : list (list B) :=
+  List.map (List.map f) ll.
+
+Inductive NoneSetPair {A B : Type} (P : A -> B -> Prop) : list A -> list B -> Prop :=
+  | NoneSP_nil : NoneSetPair P nil nil
+  | NoneSP_cons : forall x y xs ys, ~ (P x y) -> NoneSetPair P xs ys -> NoneSetPair P (x :: xs) (y :: ys).
+
+Inductive ForallSet {A : Type} (P : A -> Type) : list A -> Type :=
+| ForallS_nil : ForallSet P nil
+| ForallS_cons : forall x xs, P x -> ForallSet P xs -> ForallSet P (x :: xs).
+
+Inductive ForallSet2 {A : Type} (P : A -> Set) : list (list A) -> Type :=
+| ForallS2_nil : ForallSet2 P nil
+| ForallS2_cons : forall x xs, ForallSet P x -> ForallSet2 P xs -> ForallSet2 P (x :: xs).
+
+Inductive ForallSetPair {A B : Type} (P : A -> B -> Type) : list A -> list B -> Type :=
+| ForallSP_nil : ForallSetPair P nil nil
+| ForallSP_cons : forall x y xs ys, P x y -> ForallSetPair P xs ys -> ForallSetPair P (x :: xs) (y :: ys).
+
+Inductive ForallSetPair2 {A B : Type} (P : A -> B -> Type) : list (list A) -> list (list B) -> Type :=
+| ForallSP2_nil : ForallSetPair2 P nil nil
+| ForallSP2_cons : forall x y xs ys, ForallSetPair P x y -> ForallSetPair2 P xs ys -> ForallSetPair2 P (x :: xs) (y :: ys).
+
+Definition concat2 {A : Type} (l : list (list (list A))) : list A :=
+  List.flat_map (@List.concat A) l.
+
+(* Using convoluted fold_left version so that termination checker has a good time*)
+Definition flatmap2 {A B : Type} (f : A -> list B) (l : list (list A)) : list B :=
+  fold_left (fun (acc : list (B)) (Ts : (list (A))) => List.app acc 
+                    (fold_left (fun (acc2 : list (B)) (T : A) => List.app acc2 (f T)) Ts (nil : list (B)))
+                ) l (nil : list (B)).
